theories/Poly.v
@@ -1,0 +1,26 @@
+From ExtLib.Structures Require Import Functor Monad.
+From ITree Require Import ITree.
+From OGS Require Import Utils.
+
+Record eF (E : Type -> Type) (X : Type) := EF {
+  eF_R : Type ;
+  eF_q : E eF_R ;
+  eF_k : eF_R -> X
+}.
+
+Notation "[ E ]e" := (eF E).
+Arguments EF {E} {X} {eF_R}.
+Arguments eF_R {E} {X}.
+Arguments eF_q {E} {X}.
+Arguments eF_k {E} {X}.
+
+Definition wrap {E X} (t : [ E ]e (itree E X)) : itree E X :=
+  vis (eF_q t) (eF_k t).
+
+Instance Functor_E {E} : Functor ([ E ]e) := {|
+  fmap _ _ f := fun x => EF (eF_q x) ((f # eF_k x))
+|}. 
+
+Instance Functor_E_itree {E} : Functor ([ E ]e # itree E) := {|
+  fmap _ _ f := fun x => EF (eF_q x) (fmap f # eF_k x)
+|}.
